theories/examples/counter.v
@@ -1,0 +1,317 @@
+From iris.algebra Require Import frac.
+From iris.proofmode Require Import tactics.
+Require Import Eqdep_dec List.
+From cap_machine Require Import rules logrel macros_helpers macros fundamental.
+
+Section counter.
+  Context {Σ:gFunctors} {memg:memG Σ} {regg:regG Σ}
+          {nainv: logrel_na_invs Σ}
+          `{MP: MachineParameters}.
+
+  (* -------------------------------- LTACS -------------------------------------- *)
+  
+  (* Tactic for destructing a list into elements *)
+  Ltac destruct_list l :=
+    match goal with
+    | H : strings.length l = _ |- _ =>
+      let a := fresh "a" in
+      let l' := fresh "l" in
+      destruct l as [|a l']; [inversion H|];
+      repeat (let a' := fresh "a" in
+              destruct l' as [|a' l'];[by inversion H|]);
+      destruct l'; [|by inversion H]
+    end.
+
+  Ltac iPrologue_pre :=
+    match goal with
+    | Hlen : length ?a = ?n |- _ =>
+      let a' := fresh "a" in
+      destruct a as [| a' a]; inversion Hlen; simpl
+    end.
+
+  Ltac iPrologue prog :=
+    (try iPrologue_pre);
+    iDestruct prog as "[Hi Hprog]";
+    iApply (wp_bind (fill [SeqCtx])).
+
+  Ltac iEpilogue prog :=
+    iNext; iIntros prog; iSimpl;
+    iApply wp_pure_step_later;auto;iNext.
+
+  Ltac middle_lt prev index :=
+    match goal with
+    | Ha_first : ?a !! 0 = Some ?a_first |- _
+    => apply Z.lt_trans with prev; auto; apply incr_list_lt_succ with a index; auto
+    end.
+
+  Ltac iCorrectPC i j :=
+    eapply isCorrectPC_contiguous_range with (a0 := i) (an := j); eauto; [];
+    cbn; solve [ repeat constructor ].
+
+  Ltac iContiguous_next Ha index :=
+    apply contiguous_of_contiguous_between in Ha;
+    generalize (contiguous_spec _ Ha index); auto.
+
+  (* ----------------------------------------------------------------------------- *)
+  (* TODO: move to addr_reg_sample *)
+  Definition lt_r_z r1 r2 z := encodeInstrW (Lt r1 (inr r2) (inl z)).
+  
+
+  Definition incr_instrs :=
+    [load_r r_t1 r_env;
+    add_r_z r_t1 r_t1 1;
+    store_r r_env r_t1;
+    move_z r_env 0;
+    jmp r_t0]. 
+
+  Definition read_instrs f_a :=
+    [load_r r_t1 r_env;
+    lt_r_z r_t2 r_t1 0] ++
+    assert_r_z_instrs f_a r_t1 0 ++
+    [move_z r_env 0;
+    jmp r_t0]. 
+
+  Definition reset_instrs :=
+    [store_z r_env 0;
+    move_z r_env 0;
+    jmp r_t0].
+
+  Definition incr a :=
+    ([∗ list] a_i;w ∈ a;incr_instrs, a_i ↦ₐ w)%I.
+  Definition read a f_a :=
+    ([∗ list] a_i;w ∈ a;read_instrs f_a, a_i ↦ₐ w)%I. 
+  Definition reset a :=
+    ([∗ list] a_i;w ∈ a;reset_instrs, a_i ↦ₐ w)%I. 
+
+  Definition pos_word (w : Word) : iProp Σ :=
+    (match w with
+    | inl z => ⌜(0 < z)%Z⌝
+    | inr _ => False
+    end)%I. 
+  Definition counter_inv d : iProp Σ :=
+    (∃ w, d ↦ₐ w ∗ pos_word w)%I.
+  
+  Instance pos_word_Timeless : Timeless (pos_word w).
+  Proof. intros d. destruct d; apply _. Qed. 
+  Instance pos_word_Persistent : Persistent (pos_word w).
+  Proof. intros w. destruct w; apply _. Qed.
+
+
+  (* ----------------------------------- INCR -------------------------------------- *)
+  
+  Lemma incr_spec pc_p pc_b pc_e (* PC *)
+        wret (* return cap *)
+        incr_addrs (* program addresses *)
+        d d' (* dynamically allocated memory given by preamble *)
+        a_first a_last (* special adresses *)
+        f_a b_link e_link a_link a_entry fail_cap (* linking table variables *)
+        rmap (* registers *)
+        ι1 ι2 (* invariant names *) :
+
+    (* PC assumptions *)
+    isCorrectPC_range pc_p pc_b pc_e a_first a_last ->
+
+    (* Program adresses assumptions *)
+    contiguous_between incr_addrs a_first a_last ->
+    
+    (* Linking table assumptions *)
+    withinBounds (RW, b_link, e_link, a_entry) = true →
+    (a_link + f_a)%a = Some a_entry ->
+
+    (* malloc'ed memory assumption for the counter *)
+    (d + 1)%a = Some d' ->
+
+    (* footprint of the register map *)
+    dom (gset RegName) rmap = all_registers_s ∖ {[PC;r_t0;r_env]} →
+
+    (* The two invariants have different names *)
+    (up_close (B:=coPset) ι2 ## ↑ι1) ->
+    
+    {{{ PC ↦ᵣ inr (pc_p,pc_b,pc_e,a_first)
+      ∗ r_t0 ↦ᵣ wret
+      ∗ r_env ↦ᵣ inr (RWX,d,d',d)
+      ∗ ([∗ map] r_i↦w_i ∈ rmap, r_i ↦ᵣ w_i)
+      (* invariant for d *)
+      ∗ (∃ ι, inv ι (counter_inv d))
+      (* token which states all non atomic invariants are closed *)
+      ∗ na_own logrel_nais ⊤
+      (* callback validity *)
+      ∗ interp wret
+      (* trusted code *)
+      ∗ na_inv logrel_nais ι1 (incr incr_addrs)
+      (* linking table *)
+      ∗ na_inv logrel_nais ι2 (pc_b ↦ₐ inr (RO,b_link,e_link,a_link) ∗ a_entry ↦ₐ fail_cap)
+      (* the remaining registers are all valid *)
+      ∗ ([∗ map] _↦w_i ∈ rmap, interp w_i)
+    }}}
+      Seq (Instr Executable)
+      {{{ v, RET v; ⌜v = HaltedV⌝ →
+                    ∃ r, full_map r ∧ registers_mapsto r
+                         ∗ na_own logrel_nais ⊤ }}}.
+  Proof.
+    iIntros (Hvpc Hcont Hwb Hlink Hd Hdom Hclose φ) "(HPC & Hr_t0 & Hr_env & Hregs & Hinv & Hown & #Hcallback & #Hincr & #Hlink & #Hregs_val) Hφ". 
+    iDestruct "Hinv" as (ι) "#Hinv".
+    iMod (na_inv_open with "Hincr Hown") as "(>Hprog & Hown & Hcls)";auto.
+    iDestruct (big_sepL2_length with "Hprog") as %Hprog_length.
+    destruct_list incr_addrs.
+    apply contiguous_between_cons_inv_first in Hcont as Heq. subst a. 
+    (* Get a general purpose register *)
+    assert (is_Some (rmap !! r_t1)) as [w1 Hrt1].
+    { apply elem_of_gmap_dom. rewrite Hdom. apply elem_of_difference.
+      split;[apply all_registers_s_correct|clear;set_solver]. }
+    iDestruct (big_sepM_delete _ _ r_t1 with "Hregs") as "[Hr_t1 Hregs]";[eauto|]. 
+    (* load r_t1 r_env *)
+    iPrologue "Hprog". rewrite /counter_inv. 
+    iInv ι as (w) "[>Hd >#Hcond]" "Hcls'".
+    iAssert (⌜(d =? a_first)%a = false⌝)%I as %Hfalse.
+    { destruct (d =? a_first)%a eqn:Heq;auto. apply Z.eqb_eq,z_of_eq in Heq as ->. iDestruct (mapsto_valid_2 with "Hi Hd") as %?. done. }
+    iApply (wp_load_success with "[$HPC $Hi $Hr_t1 $Hr_env Hd]");
+      [apply decode_encode_instrW_inv|iCorrectPC a_first a_last| |iContiguous_next Hcont 0|..]. 
+    { split;auto. simpl. apply andb_true_iff. rewrite Z.leb_le Z.ltb_lt. revert Hd;clear;solve_addr. }
+    { rewrite Hfalse. iFrame. }
+    rewrite Hfalse. 
+    iNext. iIntros "(HPC & Hr_t1 & Ha_first & Hr_env & Hd)".
+    iMod ("Hcls'" with "[Hd]") as "_". 
+    { iNext. iExists w. iFrame "∗ #". }
+    iModIntro. iApply wp_pure_step_later;auto;iNext.
+    (* add r_t1 r_t1 1 *)
+    destruct w;[|done]. 
+    iPrologue "Hprog". 
+    iApply (wp_add_sub_lt_success_dst_z with "[$HPC $Hi $Hr_t1]");
+      [apply decode_encode_instrW_inv|eauto|iContiguous_next Hcont 1|iCorrectPC a_first a_last|]. 
+    iEpilogue "(HPC & Hi & Hr_t1) /=". iCombine "Hi Ha_first" as "Hprog_done". 
+    (* store r_env r_t1 *)
+    iPrologue "Hprog".
+    iInv ι as (w) "[>Hd _]" "Hcls'". 
+    iApply (wp_store_success_reg with "[$HPC $Hi $Hr_t1 $Hr_env $Hd]");
+      [apply decode_encode_instrW_inv|iCorrectPC a_first a_last|iContiguous_next Hcont 2|..]. 
+    { split;auto. simpl. apply andb_true_iff. rewrite Z.leb_le Z.ltb_lt. revert Hd;clear;solve_addr. }
+    iNext. iIntros "(HPC & Hi & Hr_t1 & Hr_env & Hd)".
+    iMod ("Hcls'" with "[Hd]") as "_". 
+    { iNext. iExists (inl (z + 1)%Z). iFrame. iDestruct "Hcond" as %Hcond. iPureIntro. revert Hcond;clear;lia. }
+    iModIntro. iApply wp_pure_step_later;auto;iNext. iCombine "Hi Hprog_done" as "Hprog_done". 
+    (* move r_env 0 *)
+    iPrologue "Hprog". 
+    iApply (wp_move_success_z with "[$HPC $Hi $Hr_env]");
+      [apply decode_encode_instrW_inv|iCorrectPC a_first a_last|iContiguous_next Hcont 3|]. 
+    iEpilogue "(HPC & Hi & Hr_env)". iCombine "Hi Hprog_done" as "Hprog_done".
+    (* jmp r_t0 *)
+    iPrologue "Hprog". 
+    apply (contiguous_between_last _ _ _ a3) in Hcont as Hlast;auto. 
+    iApply (wp_jmp_success with "[$HPC $Hi $Hr_t0]");
+      [apply decode_encode_instrW_inv|iCorrectPC a_first a_last|]. 
+    
+    (* close program invariant *)
+    
+    (* reassemble registers *)
+    iDestruct (big_sepM_insert _ _ r_t1 with "[$Hregs $Hr_t1]") as "Hregs";[apply lookup_delete|]. 
+    iDestruct (big_sepM_insert _ _ r_env with "[$Hregs $Hr_env]") as "Hregs".
+    { rewrite !lookup_insert_ne;auto. rewrite !lookup_delete_ne;auto. apply elem_of_gmap_dom_none. rewrite Hdom. clear; set_solver. }
+    (* now we are ready to apply the jump or fail pattern *)
+    destruct (decide (isCorrectPC (updatePcPerm wret))). 
+    - iDestruct "Hcallback_now" as (p b e a Heq) "Hcallback'". 
+      simplify_eq.
+      iEpilogue "(HPC & Hi & Hr_t0)".
+      iMod ("Hcls" with "[Hprog_done Hi $Hown]") as "Hown".
+      { iNext. iFrame. iDestruct "Hprog_done" as "($&$&$&$&$)". done. }
+      iDestruct (big_sepM_insert _ _ r_t0 with "[$Hregs $Hr_t0]") as "Hregs".
+      { rewrite !lookup_insert_ne;auto. rewrite !lookup_delete_ne;auto. apply elem_of_gmap_dom_none. rewrite Hdom. clear; set_solver. }
+      set (regs' := <[PC:=inl 0%Z]> (<[r_t0:=inr (p, b, e, a)]> (<[r_env:=inl 0%Z]> (<[r_t1:=inl (z + 1)%Z]> (delete r_t1 rmap))))). 
+      iDestruct ("Hcallback'" $! regs' with "[Hregs $Hown HPC]") as "[_ Hexpr]". 
+      { rewrite /registers_mapsto /regs'.
+        iSplit.
+        - iClear "Hcallback' Hregs HPC". rewrite /interp_reg /=. iSplit.
+          + iPureIntro.
+            intros r'. simpl.
+            destruct (decide (r' = PC));[subst;rewrite lookup_insert;eauto|rewrite lookup_insert_ne;auto].
+            destruct (decide (r' = r_t0));[subst;rewrite lookup_insert;eauto|rewrite lookup_insert_ne;auto].
+            destruct (decide (r' = r_env));[subst;rewrite lookup_insert;eauto|rewrite lookup_insert_ne;auto]. rewrite insert_delete. 
+            destruct (decide (r' = r_t1));[subst;rewrite lookup_insert;eauto|rewrite lookup_insert_ne;auto].
+            apply elem_of_gmap_dom. rewrite Hdom. assert (r' ∈ all_registers_s) as Hin;[apply all_registers_s_correct|].
+            revert n n0 n1 Hin;clear. set_solver.
+          + iIntros (r Hne).
+            rewrite /RegLocate. 
+            destruct (decide (r = PC));[subst;rewrite lookup_insert|rewrite lookup_insert_ne;auto]. done.
+            destruct (decide (r = r_t0));[subst;rewrite lookup_insert|rewrite lookup_insert_ne;auto]. done.
+            destruct (decide (r = r_env));[subst;rewrite lookup_insert|rewrite lookup_insert_ne;auto]. rewrite !fixpoint_interp1_eq. done.
+            destruct (decide (r = r_t1));[subst;rewrite lookup_insert|rewrite lookup_insert_ne;auto]. rewrite !fixpoint_interp1_eq. done.
+            rewrite lookup_delete_ne;auto. destruct (rmap !! r) eqn:Hsome;rewrite Hsome;[|rewrite !fixpoint_interp1_eq;done].
+            iDestruct (big_sepM_delete _ _ r with "Hregs_val") as "[Hr _]";[eauto|]. iFrame "Hr".
+        - rewrite insert_insert. iApply (big_sepM_delete _ _ PC);[apply lookup_insert|]. iFrame.
+          rewrite delete_insert. iFrame.
+          repeat (rewrite lookup_insert_ne;auto). rewrite lookup_delete_ne;auto.
+          apply elem_of_gmap_dom_none. rewrite Hdom. clear;set_solver.
+      }
+      rewrite /interp_conf. iApply wp_wand_l. iFrame "Hexpr". 
+      iIntros (v). iApply "Hφ".
+    - iEpilogue "(HPC & Hi & Hr_t0)".
+      iApply "Hcallback_now". iFrame.
+      iApply "Hφ". iIntros (Hcontr); inversion Hcontr. 
+  Qed.
+
+
+  (* ----------------------------------- READ -------------------------------------- *)
+
+  Lemma incr_spec pc_p pc_b pc_e (* PC *)
+        wret (* return cap *)
+        incr_addrs (* program addresses *)
+        d d' (* dynamically allocated memory given by preamble *)
+        a_first a_last (* special adresses *)
+        f_a b_link e_link a_link a_entry fail_cap (* linking table variables *)
+        rmap (* registers *)
+        ι1 ι2 (* invariant names *) :
+
+    (* PC assumptions *)
+    isCorrectPC_range pc_p pc_b pc_e a_first a_last ->
+
+    (* Program adresses assumptions *)
+    contiguous_between incr_addrs a_first a_last ->
+    
+    (* Linking table assumptions *)
+    withinBounds (RW, b_link, e_link, a_entry) = true →
+    (a_link + f_a)%a = Some a_entry ->
+
+    (* malloc'ed memory assumption for the counter *)
+    (d + 1)%a = Some d' ->
+
+    (* footprint of the register map *)
+    dom (gset RegName) rmap = all_registers_s ∖ {[PC;r_t0;r_env]} →
+
+    (* The two invariants have different names *)
+    (up_close (B:=coPset) ι2 ## ↑ι1) ->
+    
+    {{{ PC ↦ᵣ inr (pc_p,pc_b,pc_e,a_first)
+      ∗ r_t0 ↦ᵣ wret
+      ∗ r_env ↦ᵣ inr (RWX,d,d',d)
+      ∗ ([∗ map] r_i↦w_i ∈ rmap, r_i ↦ᵣ w_i)
+      (* invariant for d *)
+      ∗ (∃ ι, inv ι (counter_inv d))
+      (* token which states all non atomic invariants are closed *)
+      ∗ na_own logrel_nais ⊤
+      (* callback validity *)
+      ∗ interp wret
+      (* trusted code *)
+      ∗ na_inv logrel_nais ι1 (incr incr_addrs)
+      (* linking table *)
+      ∗ na_inv logrel_nais ι2 (pc_b ↦ₐ inr (RO,b_link,e_link,a_link) ∗ a_entry ↦ₐ fail_cap)
+      (* the remaining registers are all valid *)
+      ∗ ([∗ map] _↦w_i ∈ rmap, interp w_i)
+    }}}
+      Seq (Instr Executable)
+      {{{ v, RET v; ⌜v = HaltedV⌝ →
+                    ∃ r, full_map r ∧ registers_mapsto r
+                         ∗ na_own logrel_nais ⊤ }}}.
+  Proof.
+    iIntros (Hvpc Hcont Hwb Hlink Hd Hdom Hclose φ) "(HPC & Hr_t0 & Hr_env & Hregs & Hinv & Hown & #Hcallback & #Hincr & #Hlink & #Hregs_val) Hφ". 
+    iDestruct "Hinv" as (ι) "#Hinv".
+    iMod (na_inv_open with "Hincr Hown") as "(>Hprog & Hown & Hcls)";auto.
+    iDestruct (big_sepL2_length with "Hprog") as %Hprog_length.
+    destruct_list incr_addrs.
+    apply contiguous_between_cons_inv_first in Hcont as Heq. subst a. 
+    (* Get a general purpose register *)
+    assert (is_Some (rmap !! r_t1)) as [w1 Hrt1].
+    { apply elem_of_gmap_dom. rewrite Hdom. apply elem_of_difference.
+      split;[apply all_registers_s_correct|clear;set_solver]. }
+    iDestruct (big_sepM_delete _ _ r_t1 with "Hregs") as "[Hr_t1 Hregs]";[eauto|]. 
+
+  
